feat: Improved test suite

examples/scalaEquivalenceBenchmarkExamples/incomplete/unknownSafety2.dfy
@@ -1,12 +1,5 @@
 // MODEL
 
-datatype List<T> = Nil | Cons(head: T, tail: List<T>)
-
-
-function addM(x: int, y: int): int {x + y}
-
-/////////////////////////////////////
-
 function isEvenTopLvlM(x: int): bool {isEvenM(x)}
 
 function isEvenM(x: int): bool
@@ -23,35 +16,11 @@ function isOddM(x: int): bool
   else !isEvenM(x - 1)
 }
 
-/////////////////////////////////////
-
-function isSortedM(xs: List<int>): bool {
-  match xs {
-  case Nil => true
-  case Cons(_, Nil) => true
-  case Cons(h1, Cons(h2, t)) => h1 <= h2 && isSortedM(t)
-}
-}
-
-// CANDIDATE
-
-
 function zero1(x: int): int
   requires (x >= 0) {
   if (x > 0) then zero1(x - 1)
   else x
 }
-
-function add1(x: int, y: int): int {
-  if (x >= 0) then
-    var z := zero1(x);
-    assert(z == 0); // timeout
-    x + y
-  else
-    x + y
-}
-
-/////////////////////////////////////
 
 function isEvenTopLvl1(x: int): bool {isEven1(x)}
 
@@ -75,25 +44,6 @@ function isOdd1(x: int): bool
   else !isEven1(x - 1)
 }
 
-/////////////////////////////////////
-
-function isSorted1(xs: List<int>): bool {
-  match xs {
-  case Nil => true
-  case Cons(h, Nil) =>
-    if (h >= 0) then
-      assert(zero1(h) == 0); // timeout
-      true
-    else
-      true
-  case Cons(h1, Cons(h2, t)) => h1 <= h2 && isSorted1(t)
-}
-}
-
-lemma equivalence_add(x: int, y: int)
-  ensures (addM(x, y) == add1(x, y))
-{}
-
 lemma equivalence_isEven(x: int)
   ensures (isEvenM(x) == isEven1(x))
 {
@@ -115,7 +65,3 @@ lemma equivalence_isEvenTopLvl(x: int)
 {
   equivalence_isEven(x);
 }
-
-lemma equivalence_isSorted(xs: List<int>)
-  ensures (isSortedM(xs) == isSorted1(xs))
-{}
