examples/scalaEquivalenceBenchmarkExamples/separate1.dfy
@@ -33,23 +33,3 @@ lemma equivalenceSeparate1(xs: List<Animal>)
   ensures (separate1(xs) == separateM(xs))
 {}
 
-// CANDIDATE 2
-
-function separate2(xs: List<Animal>): (List<Animal>, List<Animal>) {
-  match xs {
-    case Nil => (Nil, Nil)
-    case Cons(Sheep(id), t) =>
-      var (s2, g2) := separate2(t);
-      (Cons(Sheep(id), s2), g2)
-    case Cons(Goat(id), t) =>
-      var (s2, g2) := separate2(t);
-      (s2, g2) // oops, forgets to add goat
-  }
-}
-
-// Counter Example: xs = Cons(Goat(7), Nil)
-lemma equivalenceSeparate2(xs: List<Animal>)
-  ensures (separate2(xs) == separateM(xs))
-{} 
-
-
