examples/scalaEquivalenceBenchmarkExamples/incomplete/separate2.dfy
@@ -1,0 +1,38 @@
+// MODEL
+
+datatype List<T> = Nil | Cons(head: T, tail: List<T>)
+
+datatype Animal = Sheep(id: int) | Goat(id: int)
+
+function separateM(xs: List<Animal>): (List<Animal>, List<Animal>) {
+  match xs {
+    case Nil => (Nil, Nil)
+    case Cons(Sheep(id), t) =>
+      var (s2, g2) := separateM(t);
+      (Cons(Sheep(id), s2), g2)
+    case Cons(Goat(id), t) =>
+      var (s2, g2) := separateM(t);
+      (s2, Cons(Goat(id), g2))
+  }
+}
+
+// CANDIDATE 2
+
+function separate2(xs: List<Animal>): (List<Animal>, List<Animal>) {
+  match xs {
+    case Nil => (Nil, Nil)
+    case Cons(Sheep(id), t) =>
+      var (s2, g2) := separate2(t);
+      (Cons(Sheep(id), s2), g2)
+    case Cons(Goat(id), t) =>
+      var (s2, g2) := separate2(t);
+      (s2, g2) // oops, forgets to add goat
+  }
+}
+
+// Counter Example: xs = Cons(Goat(7), Nil)
+lemma equivalenceSeparate2(xs: List<Animal>)
+  ensures (separate2(xs) == separateM(xs))
+{} 
+
+
