examples/scalaEquivalenceBenchmarkExamples/incomplete/unknownSafety3.dfy
@@ -1,0 +1,34 @@
+// MODEL
+
+datatype List<T> = Nil | Cons(head: T, tail: List<T>)
+
+function isSortedM(xs: List<int>): bool {
+  match xs {
+  case Nil => true
+  case Cons(_, Nil) => true
+  case Cons(h1, Cons(h2, t)) => h1 <= h2 && isSortedM(t)
+}
+}
+
+function zero1(x: int): int
+  requires (x >= 0) {
+  if (x > 0) then zero1(x - 1)
+  else x
+}
+
+function isSorted1(xs: List<int>): bool {
+  match xs {
+  case Nil => true
+  case Cons(h, Nil) =>
+    if (h >= 0) then
+      assert(zero1(h) == 0); // timeout
+      true
+    else
+      true
+  case Cons(h1, Cons(h2, t)) => h1 <= h2 && isSorted1(t)
+}
+}
+
+lemma equivalence_isSorted(xs: List<int>)
+  ensures (isSortedM(xs) == isSorted1(xs))
+{}
