src/test/output/separate1.dfy
@@ -1,0 +1,28 @@
+datatype Animal = Sheep(id: int) | Goat(id: int)
+
+datatype List<T> = Nil | Cons(head: T, tail: List<T>)
+
+function separateM(xs: List<Animal>): (List<Animal>, List<Animal>)
+{match xs {
+case Nil => (Nil, Nil)
+case Cons(Sheep(id), t) => var (s2, g2) := separateM(t);
+(Cons(Sheep(id), s2), g2)
+case Cons(Goat(id), t) => var (s2, g2) := separateM(t);
+(s2, Cons(Goat(id), g2))
+}
+}
+
+function separate1(xs: List<Animal>): (List<Animal>, List<Animal>)
+{match xs {
+case Nil => (Nil, Nil)
+case Cons(Sheep(id), t) => var (s2, g2) := separate1(t);
+(Cons(Sheep(id), s2), g2)
+case Cons(Goat(id), t) => var (s2, g2) := separate1(t);
+(s2, Cons(Goat(id), g2))
+}
+}
+
+lemma separate1Equivalence(xs: List<Animal>)
+ensures separateM(xs) == separate1(xs)
+{{}}
+
